src/lang/Local.v
@@ -312,16 +312,6 @@ Module Local.
     - by inv PROMISE.
   Qed.
 
-  Lemma promise_step_no_half
-        lc1 mem1 loc from to msg lc2 mem2 kind
-        (STEP: promise_step lc1 mem1 loc from to msg lc2 mem2 kind)
-        (NOHALF1: Memory.no_half lc1.(promises) mem1):
-    Memory.no_half lc2.(promises) mem2.
-  Proof.
-    ii. inv STEP. s.
-    eapply Memory.promise_no_half; eauto.
-  Qed.
-
   Lemma read_step_future lc1 mem1 loc ts val released ord lc2
         (STEP: read_step lc1 mem1 loc ts val released ord lc2)
         (WF1: wf lc1 mem1)
@@ -525,22 +515,32 @@ Module Local.
     - exploit fence_step_disjoint; eauto.
   Qed.
 
-  Lemma program_step_no_half
+  Lemma promise_step_no_half_except
+        lc1 mem1 loc from to msg lc2 mem2 kind
+        (STEP: promise_step lc1 mem1 loc from to msg lc2 mem2 kind)
+        (NOHALF1: Memory.no_half_except lc1.(promises) mem1):
+    Memory.no_half_except lc2.(promises) mem2.
+  Proof.
+    ii. inv STEP. s.
+    eapply Memory.promise_no_half_except; eauto.
+  Qed.
+
+  Lemma program_step_no_half_except
         e lc1 sc1 mem1 lc2 sc2 mem2
         (STEP: program_step e lc1 sc1 mem1 lc2 sc2 mem2)
-        (NOHALF1: Memory.no_half lc1.(promises) mem1):
-    Memory.no_half lc2.(promises) mem2.
+        (NOHALF1: Memory.no_half_except lc1.(promises) mem1):
+    Memory.no_half_except lc2.(promises) mem2.
   Proof.
     ii. inv STEP; try inv LOCAL; eauto; ss.
     - inv WRITE.
       erewrite Memory.remove_o; eauto. condtac; ss.
       + des. subst.
         exploit Memory.promise_get0; eauto. i. des. congr.
-      + eapply Memory.promise_no_half; eauto.
+      + eapply Memory.promise_no_half_except; eauto.
     - inv LOCAL1. inv LOCAL2. inv WRITE. ss.
       erewrite Memory.remove_o; eauto. condtac; ss.
       + des. subst.
         exploit Memory.promise_get0; eauto. i. des. congr.
-      + eapply Memory.promise_no_half; eauto.
+      + eapply Memory.promise_no_half_except; eauto.
   Qed.
 End Local.
